Prefix: afel: <http://vocab.afel-project.eu/>
Prefix: dc: <http://purl.org/dc/elements/1.1/>
Prefix: owl: <http://www.w3.org/2002/07/owl#>
Prefix: rdf: <http://www.w3.org/1999/02/22-rdf-syntax-ns#>
Prefix: rdfs: <http://www.w3.org/2000/01/rdf-schema#>
Prefix: xml: <http://www.w3.org/XML/1998/namespace>
Prefix: xsd: <http://www.w3.org/2001/XMLSchema#>



Ontology: <http://vocab.afel-project.eu/ont/learning>
<http://vocab.afel-project.eu/ont/learning/1.0.0>

Annotations: 
    <http://purl.org/dc/terms/contributor> "Besnik Fetahu",
    <http://purl.org/dc/terms/contributor> "Peter Holtz",
    <http://purl.org/dc/terms/creator> "Alessandro Adamou",
    <http://purl.org/dc/terms/rights> "This ontology is distributed under a Creative Commons Attribution License - http://creativecommons.org/licenses/by/3.0"@en,
    <http://purl.org/dc/terms/title> "AFEL Learning Ontology: Core module",
    rdfs:comment "A general-purpose model of learning activities, both academic and informal. This ontology is the basis for the AFEL Learning Ontology Network."@en

AnnotationProperty: <http://purl.org/dc/terms/contributor>

    
AnnotationProperty: <http://purl.org/dc/terms/creator>

    
AnnotationProperty: <http://purl.org/dc/terms/description>

    
AnnotationProperty: <http://purl.org/dc/terms/rights>

    
AnnotationProperty: <http://purl.org/dc/terms/title>

    
AnnotationProperty: rdfs:comment

    
AnnotationProperty: rdfs:isDefinedBy

    
AnnotationProperty: rdfs:label

    
AnnotationProperty: rdfs:seeAlso

    
Datatype: rdf:PlainLiteral

    
Datatype: xsd:anyURI

    
Datatype: xsd:string

    
ObjectProperty: <http://purl.org/dc/terms/hasPart>

    
ObjectProperty: afel:hasScope

    Annotations: 
        rdfs:label "has scope"@en
    
    InverseOf: 
        afel:isScopeOf
    
    
ObjectProperty: afel:hosts

    Annotations: 
        rdfs:label "hosts"@en
    
    SubPropertyOf: 
        owl:topObjectProperty
    
    InverseOf: 
        afel:isHostedOn
    
    
ObjectProperty: afel:includesActivity

    Range: 
        afel:Activity
    
    
ObjectProperty: afel:involvesUseOf

    InverseOf: 
        afel:isUsedIn
    
    
ObjectProperty: afel:isHostedOn

    Annotations: 
        rdfs:label "is hosted on"@en
    
    InverseOf: 
        afel:hosts
    
    
ObjectProperty: afel:isScopeOf

    Annotations: 
        rdfs:label "is scope of"@en
    
    InverseOf: 
        afel:hasScope
    
    
ObjectProperty: afel:isTriggeredBy

    Annotations: 
        rdfs:label "is triggered by"@en
    
    InverseOf: 
        afel:triggers
    
    
ObjectProperty: afel:isUsedIn

    Domain: 
        afel:Artifact
    
    Range: 
        afel:Activity
    
    InverseOf: 
        afel:involvesUseOf
    
    
ObjectProperty: afel:triggers

    Annotations: 
        rdfs:label "triggers"@en
    
    Range: 
        afel:Process
    
    InverseOf: 
        afel:isTriggeredBy
    
    
ObjectProperty: owl:topObjectProperty

    
Class: <http://rdfs.org/sioc/ns#Space>

    
Class: <http://schema.org/Action>

    
Class: <http://xmlns.com/foaf/0.1/Document>

    
Class: afel:Activity

    Annotations: 
        rdfs:label "activity"@en
    
    
Class: afel:ActivitySet

    SubClassOf: 
        <http://purl.org/dc/terms/hasPart> some afel:Activity,
        <http://purl.org/dc/terms/hasPart> only afel:Activity
    
    
Class: afel:Artifact

    
Class: afel:LearningActivity

    Annotations: 
        rdfs:comment "All activities – intentional or not and conscious or not – that can lead to encounters that can trigger learning processes"@en,
        rdfs:isDefinedBy <https://laglossary.github.io>,
        rdfs:label "learning activity"@en,
        rdfs:seeAlso "https://laglossary.github.io/#learning_activity"^^xsd:anyURI
    
    EquivalentTo: 
        afel:Activity
         and (afel:hasScope some afel:LearningScope)
    
    SubClassOf: 
        afel:Activity
    
    
Class: afel:LearningPath

    Annotations: 
        rdfs:isDefinedBy <https://laglossary.github.io>,
        rdfs:label "learning path"@en,
        rdfs:comment "A learning trajectory comprises “… the learning goal, the learning activities, and the thinking and learning in which the students might engage” (Martin Simon, 1995, p. 133) = what happens inside and outside the head: sum of all interactions and the processes that are triggered by these interactions."@en,
        rdfs:seeAlso "https://laglossary.github.io/#learning_trajectory"^^xsd:anyURI
    
    EquivalentTo: 
        afel:ActivitySet
         and (afel:hasScope some afel:LearningScope)
         and (afel:includesActivity only afel:LearningActivity)
    
    
Class: afel:LearningProcess

    Annotations: 
        rdfs:label "learning process"@en
    
    SubClassOf: 
        afel:Process
    
    
Class: afel:LearningScope

    Annotations: 
        rdfs:label "learning scope"@en,
        rdfs:seeAlso "https://laglossary.github.io/#learning_scope"^^xsd:anyURI,
        rdfs:isDefinedBy <https://laglossary.github.io>,
        rdfs:comment "A Learning Scope is a Scope (which is an atomic concept that might be specialised differently depending on the context) that is the scope of a Learning Trajectory. For that reason it does not specialise any class."@en
    
    EquivalentTo: 
        afel:isScopeOf some afel:LearningPath
    
    
Class: afel:Process

    
Class: afel:UserArtifactInteraction

    Annotations: 
        rdfs:comment "An action involving a learner and an artifact, potentially resulting in an occurrence of knowledge construction"@en,
        rdfs:label "user-artifact interaction"@en
    
    SubClassOf: 
        <http://schema.org/Action>
    
    
Individual: <https://laglossary.github.io>

    
DisjointClasses: 
    <http://rdfs.org/sioc/ns#Space>,<http://schema.org/Action>,afel:Activity,afel:ActivitySet,afel:Artifact,afel:Process,<http://xmlns.com/foaf/0.1/Document>

